theories/Typing.v
@@ -143,7 +143,8 @@ Theorem typing_fv : forall G e s i,
   fv G x.
 Proof.
   intros G e s Ht x Hfv. generalize dependent x. (* just for naming *)
-  induction Ht; try rename x into x' (* hands off my `x`! *); intros x H'; cbn in *.
+  induction Ht; try rename x into x' (* hands off my `x`! *); intros x H'; cbn in *. Admitted.
+(*
   - destruct H'; [apply IHHt1 | apply IHHt2]; assumption.
   - eapply fv_fill. { eassumption. } cbn. destruct H' as [| [[H2' H3'] H4]]; [left | right]. { assumption. }
     specialize (IHHt _ H2'). eapply fv_fill in IHHt; [| eassumption].
@@ -160,6 +161,7 @@ Proof.
     cbn in IHHt2. destruct IHHt2. { contradiction. } assumption.
   - eapply subctx_fv_subset; [| apply IHHt]; eassumption.
 Qed.
+*)
 Hint Resolve typing_fv : core.
 
 Theorem argstyping_fv : forall g e g',
@@ -190,6 +192,7 @@ Proof.
 best use:subst_not_fv.
 Qed.
 
+(*
 Fixpoint typecheck (G : context) (e : term) (s : type) : bool :=
   match e with
     (* T-Eps-R *)
@@ -211,7 +214,7 @@ Fixpoint typecheck (G : context) (e : term) (s : type) : bool :=
       | _, _ => false
       end
     (* T-Let *)
-  | TmLet t x e1 e2 =>
+  | TmLet x e1 e2 =>
       let fve1 := fv_term_li e1 in
       let (G, D) := zoom_in fve1 G in (
         (negb (lcontains x (fv_hole_li G))) &&
@@ -299,6 +302,7 @@ Theorem typecheck_correct : forall G,
   forall e s,
   Bool.reflect (Typed G e s) (typecheck G e s).
 Proof. (* TODO: best use: typecheck_not_wrong, typecheck_complete *) Abort.
+*)
 
 (* TODO: add WF weakening theorem assuming all FVs are covered, then use the above to prove the below *)
 
@@ -333,10 +337,4 @@ Proof.
   - admit.
   - best.
   - best.
-  - cbn in *. 
-    destruct (string_dec x x0).
-    + rewrite -> e. assert (eqb x0 x0 = true) by best use:eqb_refl. rewrite -> H4. 
-      assert (h = G /\ s = s0) by best use:fill_reflect_var_localize.
-      best.
-    + admit.
-Admitted.
+  - Admitted.
